theories/logrel/logrel.v
@@ -2,7 +2,7 @@ From iris.proofmode Require Import tactics.
 From machine_program_logic.program_logic Require Import weakestpre.
 From HypVeri.lang Require Import lang.
 From HypVeri Require Import machine_extra.
-From HypVeri.algebra Require Import base base_extra mem.
+From HypVeri.algebra Require Import base base_extra mem mailbox trans.
 Import uPred.
 
 (**  unary logical relation *)
@@ -11,12 +11,10 @@ Section logrel.
   Context `{hypparams:!HypervisorParameters}.
   Context `{vmG: !gen_VMG Σ}.
 
-
-  (* XXX: a better def using list zip? - no, gmap makes case analysis simpler*)
   Definition unknown_mem_page (p: PID) :=
     (∃ mem, ⌜∀ (a:Addr), a ∈ (addr_of_page p) -> is_Some (mem !! a)⌝ ∗ [∗ map] a ↦ w ∈ mem, (a ->a w))%I.
 
-  (** definition **)
+  (** definitions **)
 
   Context (i : (leibnizO VMID)).
 
@@ -24,47 +22,66 @@ Section logrel.
    (⌜i ≠ V0⌝ -∗
         (VMProp_holds i (1/2)%Qp -∗ WP ExecI @ i {{(λ _, True )}}))%I.
 
-  Definition pgt_own (ps: gset PID) (vo: VMID) : iProp Σ :=
-    [∗ set] p ∈ ps, p -@O> vo.
+  Definition pgt (ps: gset PID) q (vo: VMID) (be: bool) : iProp Σ :=
+    [∗ set] p ∈ ps, p -@{q}O> vo ∗ p -@{q}E> be.
 
-  Definition pgt_excl (ps: gset PID) (be: bool) : iProp Σ :=
-    [∗ set] p ∈ ps, p -@E> be.
+  (* [pagetable_entries_excl_owned]: For pages that are exclusively accessible and owned by i, i keeps the entries. *)
+  Definition pagetable_entries_excl_owned (i:VMID) (ps: gset PID) := pgt ps 1 i true.
 
-  Definition tran_half (trans: gmap Addr transaction) : iProp Σ:=
-    [∗ map] h ↦ tran ∈ trans, h -{1/2}>t tran.1.
+  (* [transaction_hpool_global_transferred]: All of half of transactions, as we don't know which one would be used by i. *)
+  (* We need the pure proposition to ensure all transaction entries are transferred.
+     Only half is needed so that the invokers can remember transactions by keeping the other half.
+     Having half of pagetable entries gives us some entra properties... [TODO] *)
+  Definition transaction_hpool_global_transferred (hpool: gset Word) (trans: gmap Addr transaction) : iProp Σ:=
+    ⌜hpool ∪ dom (gset _ ) trans = hs_all⌝ ∗ fresh_handles 1 hpool ∗
+    [∗ map] h ↦ tran ∈ trans, h -{1/2}>t tran.1 ∗ pgt tran.1.1.2 (1/2)%Qp tran.1.1.1.1.1 (bool_decide (tran.1.2 ≠ Sharing)).
 
-  Definition retri (trans: gmap Addr transaction) : iProp Σ:=
-    [∗ map] h ↦ tran ∈ trans, h ->re tran.2.
-
-  Definition pgt_own_excl_in_tran (trans: gmap Addr transaction) : iProp Σ:=
-    [∗ map] h ↦ tran ∈ trans, pgt_own tran.1.1.2 tran.1.1.1.1.1 ∗ pgt_excl tran.1.1.2 (bool_decide (tran.1.2 ≠ Sharing)).
-
-
-  Definition trans_memory_in_trans (trans : gmap Word transaction) :=
-   filter (λ kv, (kv.2.1.1.1.1.1 = i ∧ ¬(kv.2.2 = true ∧ kv.2.1.2 = Lending)) ∨ kv.2.1.1.1.2 = i) trans.
-
-  Definition trans_own_excl_transferred (trans: gmap Word transaction) :=
-    filter (λ kv, kv.2.1.2 = Donation ∧ (kv.2.1.1.1.2 = i ∨ kv.2.1.1.1.1.1 = i)) trans.
-
-  Definition trans_own_excl_owned (trans: gmap Word transaction) :=
-    filter (λ kv,  kv.2.1.1.1.1.1 = i ∧ kv.2.1.2 ≠ Donation) trans.
-
-  Definition trans_tran_transferred (trans: gmap Word transaction) :=
-    filter (λ kv, (kv.2.1.1.1.2 = i ∨ kv.2.1.1.1.1.1 = i) ∧ kv.2.1.2 = Donation) trans.
-
-  Definition trans_tran_owned (trans: gmap Addr transaction) :=
+  (* [transaction_pagetable_entries_owned]: transaction and page table entries that are owned initially by i,
+     i.e. they are not transferred by VMProp, so we doesn't need to take care of them when reasoning the primary VM.
+     As the invoker of sharing and lending transactions, i always has the ownership of involved pages.
+     Therefore, i ownes half of these pagetable entries even if they are in some transactions.
+     Furthermore, since it is suffice for the receiver to retrieve or relinquish with half of transacitons entries,
+     while the sender needs full to reclaim, we let i always own half and only pass the otner half around with VMProp*)
+  (* [TODO] properties gained, relation to [pagetable_entries_excl_owned] *)
+  Definition trans_owned (trans: gmap Word transaction) :=
     filter (λ kv, kv.2.1.1.1.1.1 = i ∧ kv.2.1.2 ≠ Donation) trans.
+  Definition transaction_pagetable_entries_owned (trans: gmap Addr transaction) : iProp Σ:=
+    [∗ map] h ↦ tran ∈ trans_owned trans, h -{1/2}>t tran.1 ∗ pgt tran.1.1.2 (1/2)%Qp tran.1.1.1.1.1 (bool_decide (tran.1.2 ≠ Sharing)).
 
-  Definition trans_retri_transferred (trans: gmap Word transaction) :=
+   (* [transaction_pagetable_entries_transferred] : For donation, the half of transaction entries that are kept by sender in case
+      of sharing and lending are also be passed around between the sender and the receiver, as retrieval in this case also requires
+      full entries.
+      Pagetable entries are transferred along as both sender and receiver could be the exclusive owner of those pages. *)
+  Definition trans_transferred (trans: gmap Word transaction) :=
+    filter (λ kv, kv.2.1.2 = Donation ∧ (kv.2.1.1.1.2 = i ∨ kv.2.1.1.1.1.1 = i)) trans.
+  Definition transaction_pagetable_entries_transferred (trans: gmap Addr transaction) : iProp Σ:=
+    [∗ map] h ↦ tran ∈ trans_transferred trans, h -{1/2}>t tran.1 ∗ pgt tran.1.1.2 1 tran.1.1.1.1.1 false.
+
+  (* [retrieval entries]: all retrieval entries of i-related transactions are required.
+     For transactions where i is the sender, we need the corresponding retrieval entries to check if it is allowed for i to reclaim,
+     for the cases when i is the receiver, they are required so that i can retrieve or relinquish *)
+  (* XXX: How to relate retrieval and transaction entries? Using option(frac_agree transaction,option bool)? or is it unnecessary? *)
+  Definition trans_retri (trans: gmap Word transaction) :=
     filter (λ kv, (kv.2.1.1.1.2 = i ∨ kv.2.1.1.1.1.1 = i)) trans.
+  Definition retrieval_entries (trans: gmap Addr transaction) : iProp Σ:=
+    [∗ map] h ↦ tran ∈ (trans_retri trans), h ->re tran.2.
 
-  Definition set_of_addr (ps:gset PID) := (set_fold (λ p (acc:gset Addr), list_to_set (addr_of_page p) ∪ acc) ∅ ps).
 
-  Definition memory_pages (ps :gset PID): iProp Σ:=
-    ∃ mem, (⌜dom (gset Addr) mem = set_of_addr ps⌝ ∗ [∗ map] k ↦ v ∈ mem, k ->a v)%I.
+  (* TODO *)
+  Definition trans_memory_in_trans (trans : gmap Word transaction) :=
+    filter (λ kv, (kv.2.1.1.1.1.1 = i ∧ ¬(kv.2.2 = true ∧ kv.2.1.2 = Lending)) ∨ kv.2.1.1.1.2 = i) trans.
 
+
+  (* TODO: we need some lemmas about it:
+     e.g. p ∈ pages_in_trans trans -> ∃h tran, trans !! h = Some tran ∧ p ∈ tran.1.1.2 *)
   Definition pages_in_trans (trans: gmap Word transaction) : gset PID :=
     map_fold (λ (k:Addr) v acc, v.1.1.2 ∪ acc) (∅: gset PID) trans.
+
+
+  (* TODO *)
+  Definition set_of_addr (ps:gset PID) := (set_fold (λ p (acc:gset Addr), list_to_set (addr_of_page p) ∪ acc) ∅ ps).
+  Definition memory_pages (ps :gset PID): iProp Σ:=
+    ∃ mem, (⌜dom (gset Addr) mem = set_of_addr ps⌝ ∗ [∗ map] k ↦ v ∈ mem, k ->a v)%I.
 
   Definition VMProp_unknown p_tx p_rx trans :=
     VMProp i
@@ -77,32 +94,25 @@ Section logrel.
                i -@{1/2}A> [ps_acc'] ∗
                LB@ i := [ps_na'] ∗
                ⌜ps_na' ## ps_acc'⌝ ∗
-               (* we need this to ensure all transaction entries are transferred *)
-               ⌜inv_trans_hpool_consistent' trans' hpool'⌝ ∗
-               ⌜{[p_rx;p_tx]} ## ps_mem_in_trans'⌝ ∗
-               (* transaction entries *)
-               hp [hpool'] ∗
-               (* All of half of transactions are required, as we don't know which one would be used by i.
-                  Only *half* is needed so that related vms can remember transactions by keeping the other half. *)
-               tran_half trans' ∗
-               tran_half (trans_tran_transferred trans') ∗
-               (tran_half (trans_tran_owned trans) -∗ tran_half (trans_tran_owned trans')) ∗
-               retri (trans_retri_transferred trans') ∗
-               (* page table entries *)
-               pgt_own_excl_in_tran (trans_own_excl_transferred trans') ∗
-               (pgt_own_excl_in_tran (trans_own_excl_owned trans) -∗ pgt_own_excl_in_tran (trans_own_excl_owned trans')) ∗
-               (pgt_own ps_oea i ∗ pgt_excl ps_oea true -∗ pgt_own ps_oea' i ∗ pgt_excl ps_oea' true) ∗
-               (* mem *)
+               (* TODO: we can dervie this from rx_page/tx_page ∗ transaction_hpool_global_transferred
+                  ⌜{[p_rx;p_tx]} ## ps_mem_in_trans''⌝ ∗ *)
+               (* transaction and pagetable entries *)
+               transaction_hpool_global_transferred hpool' trans' ∗
+               transaction_pagetable_entries_transferred trans' ∗
+               retrieval_entries trans' ∗
+               (* memory *)
                memory_pages ps_mem_in_trans' ∗
-               (memory_pages ps_oea ∗
-                memory_pages ps_mem_in_trans' -∗
-                memory_pages (ps_acc' ∖ {[p_rx;p_tx]} ∪ ps_mem_in_trans')) ∗
                R0 @@ V0 ->r encode_hvc_func(Run) ∗ R1 @@ V0 ->r encode_vmid(i) ∗
                (* status of RX *)
                RX_state@ i := rx_state ∗
-                  (* RX *)
-                  (RX@i := p_rx ∗ p_tx -@O> - ∗ p_tx -@E> true) ∗
-                  memory_pages {[p_rx]} ∗
+               (* RX *)
+               (rx_page i p_rx) ∗
+               memory_pages {[p_rx]} ∗
+               (* implication: TODO  *)
+               (transaction_pagetable_entries_owned trans -∗ transaction_pagetable_entries_owned trans') ∗
+               (* TODO : (pgt_own ps_oea i ∗ pgt_excl ps_oea true -∗ pgt_own ps_oea' i ∗ pgt_excl ps_oea' true) ∗ *)
+               (memory_pages ps_oea ∗ memory_pages ps_mem_in_trans' -∗
+                memory_pages (ps_acc' ∖ {[p_rx;p_tx]} ∪ ps_mem_in_trans')) ∗
                (* if i yielding, we give following resources back to pvm *)
                VMProp V0
                       ((∃ ps_na'' ps_acc'' trans'' hpool'',
@@ -111,19 +121,11 @@ Section logrel.
                            i -@{1/2}A> [ps_acc''] ∗
                            LB@ i := [ps_na''] ∗
                            ⌜ps_na' ## ps_acc''⌝ ∗
-                           (* we need this to ensure all transaction entries are transferred *)
-                           ⌜inv_trans_hpool_consistent' trans'' hpool''⌝ ∗
-                           ⌜{[p_rx;p_tx]} ## ps_mem_in_trans''⌝ ∗
-                           (* transaction entries *)
-                           hp [hpool''] ∗
-                           tran_half trans'' ∗
-                           tran_half (trans_tran_transferred trans'') ∗
-                           tran_half (trans_tran_owned trans'') ∗
-                           retri (trans_retri_transferred trans'') ∗
-                           (* page table entries *)
-                           pgt_own_excl_in_tran (trans_own_excl_transferred trans'') ∗
-                           pgt_own_excl_in_tran (trans_own_excl_owned trans'') ∗
-                           (* mem *)
+                           (* transaction and pagetable entries *)
+                           transaction_hpool_global_transferred hpool'' trans'' ∗
+                           transaction_pagetable_entries_transferred trans'' ∗
+                           retrieval_entries trans'' ∗
+                           (* memory *)
                            memory_pages ps_mem_in_trans'' ∗
                            R0 @@ V0 ->r encode_hvc_func(Run) ∗ R1 @@ V0 ->r encode_vmid(i) ∗
                            (* status of RX *)
@@ -132,8 +134,7 @@ Section logrel.
                               | Some _ => RX_state@ i := None ∨ RX_state@i := rx_state
                             end) ∗
                            (* RX *)
-                           (RX@i := p_rx ∗ p_tx -@O> - ∗ p_tx -@E> true) ∗
-                           memory_pages {[p_rx]})
+                           rx_page i p_rx ∗ memory_pages {[p_rx]})
                            (* no scheduling, we finish the proof *)
                            ∨ False) (1/2)%Qp
              ) (1/2)%Qp.
@@ -141,22 +142,17 @@ Section logrel.
   Program Definition interp_access ps_acc trans p_tx p_rx : iPropO Σ:=
     (
       let ps_mem_in_trans := pages_in_trans (trans_memory_in_trans trans) in
+      (* exclusively owned pages are pages i has access to, but ain't in any transactions related to i. *)
       let ps_oea := ps_acc ∖ {[p_rx;p_tx]} ∖ ps_mem_in_trans in
       (* registers *)
       (∃ regs, ⌜is_total_gmap regs⌝ ∗ [∗ map] r ↦ w ∈ regs, r @@ i ->r w) ∗
-      (* TX *)
-      (TX@i := p_tx ∗ p_tx -@O> - ∗ p_tx -@E> true ∗ memory_pages {[p_tx]}) ∗
+      (* TX page and its memory *)
+      (tx_page i p_tx ∗ memory_pages {[p_tx]}) ∗
       (* access *)
       i -@{1/2}A> [ps_acc] ∗
-      (* own & excl *)
-      pgt_own ps_oea i ∗
-      pgt_excl ps_oea true ∗
-      pgt_own_excl_in_tran (trans_own_excl_owned trans) ∗
-      (* transaction *)
-      tran_half (trans_tran_owned trans) ∗
-      (* (* mem *) *)
+      pagetable_entries_excl_owned i ps_oea ∗
+      transaction_pagetable_entries_owned trans ∗
       memory_pages ps_oea ∗
-      (* VMProp *)
       VMProp_unknown p_tx p_rx trans
       )%I.
 
